feat(jose): Add solution for Ex1.1 and move original code.

jose_solutions/Ex1.dfy
@@ -29,57 +29,81 @@ function Serialize(a : aexpr) : seq<code>
 */
 function Deserialize(cs : seq<code>) : seq<aexpr> 
 {
-  
+  DeserializeAux(cs, [])
+}
+
+function DeserializeAux(cs: seq<code>, ts: seq<aexpr>) : seq<aexpr>
+{
+  if (|cs| == 0)
+    then ts
+    else DeserializeAux(cs[1..], DeserializeCode(cs[0], ts))
+}
+
+function DeserializeCode(c: code, ts: seq<aexpr>): seq<aexpr>
+{
+  match c {
+    case VarCode(s) => [ Var(s) ] + ts
+    case ValCode(i) => [ Val(i) ] + ts
+    case UnOpCode(uop) =>
+      if (|ts| < 1)
+        then []
+        else [ UnOp(uop, ts[0]) ] + ts[1..]
+    // Since Serialize already swaps the two values, we don't need to do it here
+    // Otherwise, not commutative binary operations might be misplaced.
+    case BinOpCode(bop) => 
+      if (|ts| < 2)
+        then []
+        else [ BinOp(bop, ts[0], ts[1]) ] + ts[2..]
+  }
 }
 
 
 /*
   Ex1.2
 */
-lemma DeserializeProperty(e : aexpr)
-  ensures Deserialize(Serialize(e)) == [ e ]
-{
+// lemma DeserializeProperty(e : aexpr)
+//   ensures Deserialize(Serialize(e)) == [ e ]
+// {
  
-}
-
+// }
 
 /*
   Ex1.3
 */
-function SerializeCodes(cs : seq<code>) : seq<nat> 
-{
+// function SerializeCodes(cs : seq<code>) : seq<nat> 
+// {
 
-}
+// }
 
-function DeserializeCodes(ints : seq<nat>) : seq<code> {
+// function DeserializeCodes(ints : seq<nat>) : seq<code> {
   
-}
+// }
 
 
 /*
   Ex1.4
 */
-lemma DeserializeCodesProperty(cs : seq<code>)
-  ensures DeserializeCodes(SerializeCodes(cs)) == cs
-{
-}
+// lemma DeserializeCodesProperty(cs : seq<code>)
+//   ensures DeserializeCodes(SerializeCodes(cs)) == cs
+// {
+// }
 
 /*
   Ex1.5
 */
-function FullSerialize(e : aexpr) : seq<nat> {
+// function FullSerialize(e : aexpr) : seq<nat> {
  
-}
+// }
 
-function FullDeserealize(nats : seq<nat>) : seq<aexpr> {
+// function FullDeserealize(nats : seq<nat>) : seq<aexpr> {
  
-}
+// }
 
 /*
   Ex1.6
 */
-lemma FullDeserealizeProperty(e : aexpr)
-  ensures FullDeserealize(FullSerialize(e)) == [ e ]
-{
+// lemma FullDeserealizeProperty(e : aexpr)
+//   ensures FullDeserealize(FullSerialize(e)) == [ e ]
+// {
     
-}
+// }
