original/Ex1.dfy
@@ -1,0 +1,85 @@
+datatype uop = Neg 
+datatype bop = Plus | Minus 
+
+datatype aexpr =
+  Var(seq<nat>)
+  | Val(nat)
+  | UnOp(uop, aexpr)
+  | BinOp(bop, aexpr, aexpr)
+ 
+datatype code = 
+  | VarCode(seq<nat>)  
+  | ValCode(nat)       
+  | UnOpCode(uop)      
+  | BinOpCode(bop)     
+
+function Serialize(a : aexpr) : seq<code> 
+{
+  match a {
+    case Var(s) => [ VarCode(s) ]
+    case Val(i) => [ ValCode(i) ]
+    case UnOp(op, a1) => Serialize(a1) + [ UnOpCode(op) ]
+    case BinOp(op, a1, a2) => Serialize(a2) + Serialize(a1) + [ BinOpCode(op) ]
+  }
+}
+
+
+/*
+  Ex1.1
+*/
+function Deserialize(cs : seq<code>) : seq<aexpr> 
+{
+  
+}
+
+
+/*
+  Ex1.2
+*/
+lemma DeserializeProperty(e : aexpr)
+  ensures Deserialize(Serialize(e)) == [ e ]
+{
+ 
+}
+
+
+/*
+  Ex1.3
+*/
+function SerializeCodes(cs : seq<code>) : seq<nat> 
+{
+
+}
+
+function DeserializeCodes(ints : seq<nat>) : seq<code> {
+  
+}
+
+
+/*
+  Ex1.4
+*/
+lemma DeserializeCodesProperty(cs : seq<code>)
+  ensures DeserializeCodes(SerializeCodes(cs)) == cs
+{
+}
+
+/*
+  Ex1.5
+*/
+function FullSerialize(e : aexpr) : seq<nat> {
+ 
+}
+
+function FullDeserealize(nats : seq<nat>) : seq<aexpr> {
+ 
+}
+
+/*
+  Ex1.6
+*/
+lemma FullDeserealizeProperty(e : aexpr)
+  ensures FullDeserealize(FullSerialize(e)) == [ e ]
+{
+    
+}
